src/cbor/spec/raw/CBOR.Spec.API.Type.fst
@@ -1,425 +1,102 @@
 module CBOR.Spec.API.Type
 
+module RF = CBOR.Spec.Raw.Format
 module R = CBOR.Spec.Raw.Sort
+module DM = CBOR.Spec.Raw.DataModel
 
-let cbor_bool (x: R.raw_data_item) : Tot bool =
-  R.raw_data_item_ints_optimal x &&
-  R.raw_data_item_sorted R.deterministically_encoded_cbor_map_key_order x
+unfold let order = RF.deterministically_encoded_cbor_map_key_order
 
-let cbor_prop (x: R.raw_data_item) : Tot prop =
-  cbor_bool x == true
+unfold let compare : (compare: (R.raw_data_item -> R.raw_data_item -> int) { R.compare_prop order compare })
+=
+  RF.cbor_compare
 
-let cbor = (x: R.raw_data_item { cbor_prop x })
+let cbor = DM.cbor order compare
 
-unfold
-let cbor_map_prop (x: list (R.raw_data_item & R.raw_data_item)) : Tot prop =
-  List.Tot.for_all (U.holds_on_pair R.raw_data_item_ints_optimal) x == true /\
-  List.Tot.for_all (U.holds_on_pair (R.raw_data_item_sorted R.deterministically_encoded_cbor_map_key_order)) x == true /\
-  List.Tot.sorted (R.map_entry_order R.deterministically_encoded_cbor_map_key_order _) x
+let cbor_map = DM.cbor_map order compare
 
-let cbor_map = (x: list (R.raw_data_item & R.raw_data_item) { cbor_map_prop x })
+let cbor_map_get = DM.cbor_map_get
 
-let list_assoc_cbor
-  (m: cbor_map)
-  (k: R.raw_data_item)
-: Lemma
-  (requires (Some? (List.Tot.assoc k m)))
-  (ensures (match List.Tot.assoc k m with
-  | None -> False
-  | Some v ->
-    cbor_prop k /\ cbor_prop v
-  ))
-= let Some v = List.Tot.assoc k m in
-  List.Tot.assoc_memP_some k v m;
-  List.Tot.for_all_mem (U.holds_on_pair R.raw_data_item_ints_optimal) m;
-  List.Tot.for_all_mem (U.holds_on_pair (R.raw_data_item_sorted R.deterministically_encoded_cbor_map_key_order)) m
+let cbor_map_get_precedes = DM.cbor_map_get_precedes
 
-let cbor_map_get m k =
-  match List.Tot.assoc k m with
-  | None -> None
-  | Some v ->
-    list_assoc_cbor m k;
-    Some v
-
-let cbor_map_get_precedes m k =
-  match List.Tot.assoc k m with
-  | None -> ()
-  | Some v ->
-    CBOR.Spec.Util.list_assoc_mem_intro k v m;
-    List.Tot.memP_precedes (k, v) m
+let cbor_map_equal_eq (m1 m2: cbor_map) : Lemma
+  (ensures DM.cbor_map_equal m1 m2 <==> cbor_map_equal m1 m2)
+//  [SMTPat (cbor_map_equal m1 m2)]
+= assert_norm (DM.cbor_map_equal m1 m2 <==> cbor_map_equal m1 m2) // FIXME: WHY WHY WHY?
 
 let cbor_map_ext m1 m2 =
-  let prf () : Lemma
-    (requires (cbor_map_equal m1 m2))
-    (ensures (m1 == m2))
-  =
-    R.deterministically_encoded_cbor_map_key_order_assoc_ext m1 m2 (fun k ->
-      match List.Tot.assoc k m1, List.Tot.assoc k m2 with
-      | Some v, _ ->
-        list_assoc_cbor m1 k;
-        assert (cbor_map_get m1 k == cbor_map_get m2 k)
-      | _, Some v ->
-        list_assoc_cbor m2 k;
-        assert (cbor_map_get m1 k == cbor_map_get m2 k)
-      | _ -> ()
-    )
-  in
-  Classical.move_requires prf ()
+  cbor_map_equal_eq m1 m2;
+  DM.cbor_map_ext m1 m2
 
-let rec cbor_map_set_keys m =
-  match m with
-  | [] -> FS.emptyset
-  | (a, _) :: q -> FS.union (FS.singleton a) (cbor_map_set_keys q)
+let cbor_map_set_keys = DM.cbor_map_set_keys
 
-let rec cbor_map_set_keys_mem m k =
-  match m with
-  | [] -> ()
-  | (a, _) :: q ->
-    if k = a
-    then ()
-    else cbor_map_set_keys_mem q k
+let cbor_map_set_keys_mem = DM.cbor_map_set_keys_mem
 
-let rec cbor_map_length m =
-  match m with
-  | [] -> 0
-  | kv :: q ->
-    let (a, _) = kv in
-    let s' = cbor_map_set_keys q in
-    let prf : squash (FS.mem a s' == false) =
-      if FS.mem a s'
-      then begin
-        let Some v' = List.Tot.assoc a q in
-        List.Tot.assoc_memP_some a v' q;
-        U.list_sorted_memP (R.map_entry_order R.deterministically_encoded_cbor_map_key_order _) kv q (a, v')
-      end
-      else ()
-    in
-    1 + cbor_map_length q
+let cbor_map_length = DM.cbor_map_length
 
-let rec cbor_map_length_eq
-  (m: cbor_map)
-: Lemma
-  (cbor_map_length m == List.Tot.length m)
-= match m with
-  | [] -> ()
-  | _ :: q -> cbor_map_length_eq q
+let cbor_map_empty = DM.cbor_map_empty
 
-let cbor_map_empty = []
+let cbor_map_get_empty = DM.cbor_map_get_empty
 
-let cbor_map_get_empty _ = ()
+let cbor_map_singleton = DM.cbor_map_singleton
 
-let cbor_map_singleton k v = [k, v]
+let cbor_map_get_singleton = DM.cbor_map_get_singleton
 
-let cbor_map_get_singleton k v k' = ()
+let cbor_map_filter = DM.cbor_map_filter
 
-let cbor_map_filter_f
-  (f: (cbor & cbor) -> bool)
-  (x: (R.raw_data_item & R.raw_data_item))
-: Tot bool =
-    if cbor_bool (fst x) && cbor_bool (snd x)
-    then f (fst x, snd x)
-    else false
+let cbor_map_get_filter = DM.cbor_map_get_filter
 
-let cbor_map_filter f m =
-  U.list_sorted_filter (R.map_entry_order R.deterministically_encoded_cbor_map_key_order _) (cbor_map_filter_f f) m;
-  List.Tot.filter (cbor_map_filter_f f) m
+let cbor_map_length_filter = DM.cbor_map_length_filter
 
-let rec cbor_map_get_filter'
-  (f: (cbor & cbor -> bool))
-  (m: cbor_map)
-  (k: cbor)
-: Lemma
-  (ensures (cbor_map_get (cbor_map_filter f m) k == begin match cbor_map_get m k with
-  | None -> None
-  | Some v -> if f (k, v) then Some v else None
-  end))
-  (decreases m)
-= match m with
-  | [] -> ()
-  | (a, v) :: q ->
-    if k = a
-    then begin
-      if f (k, v)
-      then ()
-      else begin
-        match cbor_map_get (cbor_map_filter f q) k with
-        | None -> ()
-        | Some v' ->
-          List.Tot.assoc_memP_some a v' (cbor_map_filter f q);
-          U.list_sorted_memP (R.map_entry_order R.deterministically_encoded_cbor_map_key_order _) (a, v) q (a, v')
-      end
-    end
-    else cbor_map_get_filter' f q k
+let cbor_map_union = DM.cbor_map_union
 
-let cbor_map_get_filter = cbor_map_get_filter'
+let cbor_map_get_union = DM.cbor_map_get_union
 
-let cbor_map_diff_f (m1: cbor_map) (kv: (cbor & cbor)) : Tot bool =
-  None? (cbor_map_get m1 (fst kv))
+let cbor_map_key_list = DM.cbor_map_key_list
 
-let cbor_map_length_filter f m =
-  cbor_map_length_eq m;
-  cbor_map_length_eq (cbor_map_filter f m);
-  U.list_length_filter (cbor_map_filter_f f) m
+let cbor_map_key_list_mem = DM.cbor_map_key_list_mem
 
-let cbor_map_union m1 m2 =
-  let m2' = cbor_map_filter (cbor_map_diff_f m1) m2 in
-  List.Tot.for_all_mem (U.holds_on_pair R.raw_data_item_ints_optimal) m1;
-  List.Tot.for_all_mem (U.holds_on_pair R.raw_data_item_ints_optimal) m2';
-  List.Tot.for_all_mem (U.holds_on_pair (R.raw_data_item_sorted R.deterministically_encoded_cbor_map_key_order)) m1;
-  List.Tot.for_all_mem (U.holds_on_pair (R.raw_data_item_sorted R.deterministically_encoded_cbor_map_key_order)) m2';
-  Classical.forall_intro (List.Tot.append_memP m1 m2');
-  let m' = m1 `List.Tot.append` m2' in
-  CBOR.Spec.Raw.Map.list_sorted_map_entry_order_no_repeats R.deterministically_encoded_cbor_map_key_order m1;
-  CBOR.Spec.Raw.Map.list_sorted_map_entry_order_no_repeats R.deterministically_encoded_cbor_map_key_order m2';
-  assert (List.Tot.no_repeats_p (List.Tot.map fst m1));
-  assert (List.Tot.no_repeats_p (List.Tot.map fst m2'));
-  let prf
-    (x: R.raw_data_item)
-  : Lemma
-    (requires (List.Tot.memP x (List.Tot.map fst m1)))
-    (ensures (~ (List.Tot.memP x (List.Tot.map fst m2'))))
-  = List.Tot.assoc_mem x m1;
-    List.Tot.assoc_mem x m2';
-    if Some? (List.Tot.assoc x m2')
-    then begin
-      list_assoc_cbor m2' x;
-      cbor_map_get_filter (cbor_map_diff_f m1) m2' x
-    end
-  in
-  Classical.forall_intro (Classical.move_requires prf);
-  List.Tot.no_repeats_p_append (List.Tot.map fst m1) (List.Tot.map fst m2');
-  List.Tot.map_append fst m1 m2';
-  let res = R.cbor_map_sort_failsafe m' in
-  List.Tot.for_all_mem (U.holds_on_pair R.raw_data_item_ints_optimal) res;
-  List.Tot.for_all_mem (U.holds_on_pair (R.raw_data_item_sorted R.deterministically_encoded_cbor_map_key_order)) res;
-  res
+let cbor_map_key_list_no_repeats_p = DM.cbor_map_key_list_no_repeats_p
 
-let cbor_map_get_union m1 m2 k =
-  let m2' = cbor_map_filter (cbor_map_diff_f m1) m2 in
-  R.cbor_map_sort_failsafe_correct (List.Tot.append m1 m2');
-  CBOR.Spec.Raw.Map.list_sorted_map_entry_order_no_repeats R.deterministically_encoded_cbor_map_key_order (cbor_map_union m1 m2);
-  U.list_assoc_append k m1 m2';
-  cbor_map_get_filter (cbor_map_diff_f m1) m2 k
+let cbor_map_key_list_length = DM.cbor_map_key_list_length
 
-let cast_to_cbor (x: R.raw_data_item) : Tot cbor =
-  if cbor_bool x
-  then x
-  else R.Simple 0uy // dummy
+let cbor_map_fold = DM.cbor_map_fold
 
-let list_cbor_of_cbor_list
-  (l: list R.raw_data_item)
-: Tot (list cbor)
-= List.Tot.map cast_to_cbor l
+let cbor_map_fold_ext = DM.cbor_map_fold_ext
 
-// let cbor_map_key_list_raw (m: cbor_map) : Tot (list R.raw_data_item) = List.Tot.map fst m
+let cbor_map_fold_eq = DM.cbor_map_fold_eq
 
-let rec cbor_map_key_list_tot (m: cbor_map) : Tot (list cbor) =
-  match m with
-  | [] -> []
-  | (k, _) :: q -> k :: cbor_map_key_list_tot q
+let cbor_map_fold_eq_idem = DM.cbor_map_fold_eq_idem
 
-let cbor_map_key_list (m: cbor_map) : GTot (list cbor) =
-  cbor_map_key_list_tot m
-
-let rec cbor_map_key_list_mem_aux (m: cbor_map) (k: cbor) : Lemma
-  (List.Tot.memP k (cbor_map_key_list m) <==> List.Tot.memP k (List.Tot.map fst m))
-= match m with
-  | [] -> ()
-  | (k', _) :: q ->
-    if k = k' then () else cbor_map_key_list_mem_aux q k
-
-let cbor_map_key_list_mem (m: cbor_map) (k: cbor) : Lemma
-  (List.Tot.memP k (cbor_map_key_list m) <==> cbor_map_defined k m)
-= cbor_map_key_list_mem_aux m k;
-  List.Tot.assoc_mem k m;
-  List.Tot.mem_memP k (List.Tot.map fst m)
-
-let rec cbor_map_key_list_no_repeats_p (m: cbor_map) : Lemma
-  (List.Tot.no_repeats_p (cbor_map_key_list m))
-= CBOR.Spec.Raw.Map.list_sorted_map_entry_order_no_repeats R.deterministically_encoded_cbor_map_key_order m;
-  match m with
-  | [] -> ()
-  | (k, _) :: q ->
-    cbor_map_key_list_mem_aux q k;
-    cbor_map_key_list_no_repeats_p q
-
-let rec cbor_map_key_list_length (m: cbor_map) : Lemma
-  (List.Tot.length (cbor_map_key_list m) == cbor_map_length m)
-= match m with
-  | [] -> ()
-  | _ :: q -> cbor_map_key_list_length q
-
-let cbor_map_fold
-  (#a: Type)
-  (f: a -> cbor -> a)
-  (x: a)
-  (m: cbor_map)
-: Tot a
-= List.Tot.fold_left f x (cbor_map_key_list_tot m)
-
-let rec list_sorted_map_entry_order
-  (#key #value: Type)
-  (f: key -> key -> bool {
-    U.order_irrefl f /\
-    U.order_trans f
-  })
-  (l: list (key & value))
-: Lemma
-  (requires (List.Tot.sorted (R.map_entry_order f value) l))
-  (ensures (List.Tot.sorted f (List.Tot.map fst l)))
-= match l with
-  | [] -> ()
-  | a :: q -> list_sorted_map_entry_order f q
-
-let rec cbor_map_key_list_sorted
-  (m: cbor_map)
-: Lemma
-  (List.Tot.sorted R.deterministically_encoded_cbor_map_key_order (cbor_map_key_list m))
-= list_sorted_map_entry_order R.deterministically_encoded_cbor_map_key_order m;
-  match m with
-  | [] -> ()
-  | a :: q ->
-    cbor_map_key_list_sorted q
-
-let cbor_map_fold_ext
-  (#a: Type)
-  (f1 f2: a -> cbor -> a)
-  (x: a)
-  (m1 m2: cbor_map)
-= let l1 = cbor_map_key_list m1 in
-  cbor_map_key_list_sorted m1;
-  cbor_map_key_list_sorted m2;  
-  U.list_sorted_ext_eq R.deterministically_encoded_cbor_map_key_order l1 (cbor_map_key_list m2);
-  U.list_fold_ext f1 f2 x l1
-
-let cbor_map_fold_eq
-  (#a: Type)
-  (f: a -> cbor -> a)
-  (x: a)
-  (m: cbor_map)
-  (l: list cbor)
-: Lemma
-  (requires (
-    U.op_comm f /\
-    (forall (x: cbor) . List.Tot.memP x l <==> cbor_map_defined x m) /\
-    List.Tot.no_repeats_p l
-  ))
-  (ensures (
-    cbor_map_fold f x m == List.Tot.fold_left f x l
-  ))
-= cbor_map_key_list_no_repeats_p m;
-  U.list_fold_ext_no_repeats_p f x (cbor_map_key_list m) l
-
-let cbor_map_fold_eq_idem
-  (#a: Type)
-  (f: a -> cbor -> a)
-  (x: a)
-  (m: cbor_map)
-  (l: list cbor)
-= U.list_fold_ext_idem f x (cbor_map_key_list m) l
-
-let rec cbor_list_of_list_cbor_precedes (l: list R.raw_data_item {
-    List.Tot.for_all (R.holds_on_raw_data_item R.raw_data_item_ints_optimal_elem) l /\
-    List.Tot.for_all (R.holds_on_raw_data_item (R.raw_data_item_sorted_elem R.deterministically_encoded_cbor_map_key_order)) l
-  }) (x: cbor) : Lemma
-  (requires (
-    List.Tot.memP x (list_cbor_of_cbor_list l)
-  ))
-  (ensures (x << l))
-= let a :: q = l in
-  if a = x
-  then ()
-  else (
-    assert (q << l);
-    cbor_list_of_list_cbor_precedes q x
-  )
+let unpack_aux
+  (x' : DM.cbor_case order compare)
+: cbor_case
+=
+  match x' with
+  | DM.CSimple v -> CSimple v
+  | DM.CInt64 ty v -> CInt64 ty v
+  | DM.CString ty v -> CString ty v
+  | DM.CArray v -> CArray v
+  | DM.CMap c -> CMap c
+  | DM.CTagged tag v -> CTagged tag v
 
 let unpack m =
-  assert_norm (R.raw_data_item_ints_optimal == R.holds_on_raw_data_item R.raw_data_item_ints_optimal_elem);
-  assert_norm (R.raw_data_item_sorted R.deterministically_encoded_cbor_map_key_order == R.holds_on_raw_data_item (R.raw_data_item_sorted_elem R.deterministically_encoded_cbor_map_key_order));
-  R.holds_on_raw_data_item_eq R.raw_data_item_ints_optimal_elem m;
-  R.holds_on_raw_data_item_eq (R.raw_data_item_sorted_elem R.deterministically_encoded_cbor_map_key_order) m;
-  match m with
-  | R.Simple v -> CSimple v
-  | R.Int64 ty v -> CInt64 ty v.value
-  | R.String ty len v -> CString ty v
-  | R.Array len v -> CArray (list_cbor_of_cbor_list v)
-  | R.Map len v ->
-    cbor_map_length_eq v;
-    CMap v
-  | R.Tagged tag v -> CTagged tag.value v
+  unpack_aux (DM.unpack m)
 
-let cast_from_cbor (x: cbor) : Tot R.raw_data_item = x
+let pack_aux (x: cbor_case)
+: Tot (DM.cbor_case order compare)
+=
+  match x with
+  | CSimple v -> DM.CSimple v
+  | CInt64 ty v -> DM.CInt64 ty v
+  | CString ty v -> DM.CString ty v
+  | CArray v -> DM.CArray v
+  | CMap c -> DM.CMap c
+  | CTagged tag v -> DM.CTagged tag v
+  
+let pack x = DM.pack (pack_aux x)
 
-let cbor_list_of_list_cbor (l: list cbor) : Tot (list R.raw_data_item) =
-  List.Tot.map cast_from_cbor l
+let unpack_pack c = DM.unpack_pack (pack_aux c)
 
-let cbor_list_of_list_cbor_correct
-  (l: list cbor)
-: Lemma
-  (ensures (let l' = cbor_list_of_list_cbor l in
-   List.Tot.for_all (R.holds_on_raw_data_item R.raw_data_item_ints_optimal_elem) l' == true /\
-   List.Tot.for_all (R.holds_on_raw_data_item (R.raw_data_item_sorted_elem R.deterministically_encoded_cbor_map_key_order)) l' == true
-  ))
-  [SMTPat (cbor_list_of_list_cbor l)]
-= U.list_for_all_truep l;
-  assert_norm (R.raw_data_item_ints_optimal == R.holds_on_raw_data_item R.raw_data_item_ints_optimal_elem);
-  assert_norm (R.raw_data_item_sorted R.deterministically_encoded_cbor_map_key_order == R.holds_on_raw_data_item (R.raw_data_item_sorted_elem R.deterministically_encoded_cbor_map_key_order));
-  U.list_for_all_map cast_from_cbor l U.truep R.raw_data_item_ints_optimal (fun _ -> ());
-  U.list_for_all_map cast_from_cbor l U.truep (R.raw_data_item_sorted R.deterministically_encoded_cbor_map_key_order)  (fun _ -> ())
+let pack_unpack c = DM.pack_unpack c
 
-let pack x =
-  let m : R.raw_data_item = match x with
-  | CSimple v -> R.Simple v
-  | CInt64 ty v -> R.Int64 ty (R.mk_raw_uint64 v)
-  | CString ty v -> R.String ty (R.mk_raw_uint64 (U64.uint_to_t (Seq.length v))) v
-  | CArray v -> R.Array (R.mk_raw_uint64 (U64.uint_to_t (List.Tot.length v))) (cbor_list_of_list_cbor v)
-  | CMap v ->
-    cbor_map_length_eq v;
-    R.Map (R.mk_raw_uint64 (U64.uint_to_t (List.Tot.length v))) v
-  | CTagged tag v -> R.Tagged (R.mk_raw_uint64 tag) v
-  in
-  assert_norm (R.raw_data_item_ints_optimal == R.holds_on_raw_data_item R.raw_data_item_ints_optimal_elem);
-  assert_norm (R.raw_data_item_sorted R.deterministically_encoded_cbor_map_key_order == R.holds_on_raw_data_item (R.raw_data_item_sorted_elem R.deterministically_encoded_cbor_map_key_order));
-  R.holds_on_raw_data_item_eq R.raw_data_item_ints_optimal_elem m;
-  R.holds_on_raw_data_item_eq (R.raw_data_item_sorted_elem R.deterministically_encoded_cbor_map_key_order) m;
-  m
-
-let rec cbor_list_of_list_cbor_of_cbor_list
-  (l: list R.raw_data_item {
-    List.Tot.for_all (R.holds_on_raw_data_item R.raw_data_item_ints_optimal_elem) l == true /\
-    List.Tot.for_all (R.holds_on_raw_data_item (R.raw_data_item_sorted_elem R.deterministically_encoded_cbor_map_key_order)) l == true
-  })
-: Lemma
-  (cbor_list_of_list_cbor (list_cbor_of_cbor_list l) == l)
-= match l with
-  | [] -> ()
-  | _ :: q -> cbor_list_of_list_cbor_of_cbor_list q
-
-let rec list_cbor_of_cbor_list_of_list_cbor
-  (l: list cbor)
-: Lemma
-  (list_cbor_of_cbor_list (cbor_list_of_list_cbor l) == l)
-= match l with
-  | [] -> ()
-  | _ :: q -> list_cbor_of_cbor_list_of_list_cbor q
-
-let unpack_pack c = match c with
-  | CArray v -> list_cbor_of_cbor_list_of_list_cbor v
-  | _ -> ()
-
-let pack_unpack c = match c with
-  | R.Simple _ -> ()
-  | R.Int64 _ v
-  | R.Tagged v _
-  | R.Map v _
-  | R.String _ v _ -> R.raw_uint64_optimal_unique v (R.mk_raw_uint64 v.value)
-  | R.Array len v ->
-    R.raw_uint64_optimal_unique len (R.mk_raw_uint64 len.value);
-    cbor_list_of_list_cbor_of_cbor_list v
-
-let unpack_precedes c =
-  match c with
-  | R.Array _ v ->
-    Classical.forall_intro (Classical.move_requires (cbor_list_of_list_cbor_precedes v))
-  | _ -> ()
+let unpack_precedes c = DM.unpack_precedes c
