src/cbor/spec/raw/CBOR.Spec.Raw.Sort.fsti
@@ -1,67 +1,95 @@
 module CBOR.Spec.Raw.Sort
 include CBOR.Spec.Raw.Optimal
-include CBOR.Spec.Raw.Format
 open CBOR.Spec.Util
+
+let compare_prop
+  (order: raw_data_item -> raw_data_item -> bool)
+  (compare: raw_data_item -> raw_data_item -> int)
+: Tot prop
+=
+    (forall x . order x x == false) /\
+    (forall x y z . (order x y /\ order y z) ==> order x z) /\
+    (forall x y . order x y == (compare x y < 0)) /\
+    (forall x y . compare x y == 0 <==> x == y) /\
+    (forall x y . (compare x y < 0 <==> compare y x > 0))
 
 noextract [@@noextract_to "krml"]
 val cbor_map_sort
+  (order: raw_data_item -> raw_data_item -> bool)
   (l: list (raw_data_item & raw_data_item))
 : Tot (list (raw_data_item & raw_data_item))
 
 val cbor_map_sort_correct
+  (order: raw_data_item -> raw_data_item -> bool)
+  (compare: raw_data_item -> raw_data_item -> int {
+    compare_prop order compare
+  })
   (l: list (raw_data_item & raw_data_item))
 : Lemma
   (requires List.Tot.no_repeats_p (List.Tot.map fst l))
-  (ensures (let l' = cbor_map_sort l in
+  (ensures (let l' = cbor_map_sort order l in
     List.Tot.length l' == List.Tot.length l /\
     (forall x . List.Tot.memP x l' <==> List.Tot.memP x l) /\
     (List.Tot.no_repeats_p (List.Tot.map fst l')) /\
-    List.Tot.sorted (map_entry_order deterministically_encoded_cbor_map_key_order _) l' /\
+    List.Tot.sorted (map_entry_order order _) l' /\
     (forall k . List.Tot.assoc k l' == List.Tot.assoc k l)
   ))
-  [SMTPat (cbor_map_sort l)]
 
 let cbor_map_sort_failsafe
+  (order: raw_data_item -> raw_data_item -> bool)
   (l: list (raw_data_item & raw_data_item))
 : Tot (list (raw_data_item & raw_data_item))
 = if List.Tot.noRepeats (List.Tot.map fst l)
-  then cbor_map_sort l
+  then cbor_map_sort order l
   else l
 
 let cbor_map_sort_failsafe_correct
+  (order: raw_data_item -> raw_data_item -> bool)
+  (compare: raw_data_item -> raw_data_item -> int {
+    compare_prop order compare
+  })
   (l: list (raw_data_item & raw_data_item))
 : Lemma
-  (let l' = cbor_map_sort_failsafe l in
+  (let l' = cbor_map_sort_failsafe order l in
     List.Tot.length l' == List.Tot.length l /\
     (forall x . List.Tot.memP x l' <==> List.Tot.memP x l) /\
     (List.Tot.no_repeats_p (List.Tot.map fst l') <==> List.Tot.no_repeats_p (List.Tot.map fst l)) /\
     (List.Tot.no_repeats_p (List.Tot.map fst l) ==> (
-      List.Tot.sorted (map_entry_order deterministically_encoded_cbor_map_key_order _) l' /\
+      List.Tot.sorted (map_entry_order order _) l' /\
       List.Tot.no_repeats_p (List.Tot.map fst l') /\
       (forall k . List.Tot.assoc k l' == List.Tot.assoc k l)
     ))
   )
-= ()
+= Classical.move_requires (cbor_map_sort_correct order compare) l
 
 let cbor_raw_sort_elem
+  (order: raw_data_item -> raw_data_item -> bool)
+  (compare: raw_data_item -> raw_data_item -> int {
+    compare_prop order compare
+  })
   (x: raw_data_item)
 : Tot raw_data_item
-= match x with
-  | Map len v -> Map len (cbor_map_sort_failsafe v)
+= Classical.forall_intro (cbor_map_sort_failsafe_correct order compare);
+  match x with
+  | Map len v -> Map len (cbor_map_sort_failsafe order v)
   | _ -> x
 
-let cbor_raw_sort = raw_data_item_fmap cbor_raw_sort_elem
+let cbor_raw_sort order compare = raw_data_item_fmap (cbor_raw_sort_elem order compare)
 
 val cbor_raw_sort_correct
+  (order: raw_data_item -> raw_data_item -> bool)
+  (compare: raw_data_item -> raw_data_item -> int {
+    compare_prop order compare
+  })
   (x: raw_data_item)
 : Lemma
   (requires (raw_data_item_ints_optimal x == true /\
     valid_raw_data_item x == true
   ))
   (ensures (
-    let x' = cbor_raw_sort x in
+    let x' = cbor_raw_sort order compare x in
     raw_data_item_ints_optimal x' == true /\
-    raw_data_item_sorted deterministically_encoded_cbor_map_key_order x' == true /\
+    raw_data_item_sorted order x' == true /\
     valid_raw_data_item x'  == true /\
     raw_equiv x x' /\
     begin match x, x' with
