src/cbor/pulse/raw/everparse/CBOR.Pulse.Raw.Format.Parse.fst
@@ -372,6 +372,8 @@ fn split_nondep_then_tot_kind
 module GR = Pulse.Lib.GhostReference
 module Ref = Pulse.Lib.Reference
 
+#push-options "--z3rlimit 32"
+
 #restart-solver
 fn cbor_raw_sorted (sq: squash SZ.fits_u64) : LowParse.Pulse.Recursive.impl_pred_t u#0 u#0 #_ serialize_raw_data_item_param (R.raw_data_item_sorted_elem deterministically_encoded_cbor_map_key_order)
 = (a: _)
@@ -524,6 +526,8 @@ fn cbor_raw_sorted (sq: squash SZ.fits_u64) : LowParse.Pulse.Recursive.impl_pred
     true
   }
 }
+
+#pop-options
 
 #restart-solver
 
